module Ind where

import Relation.Binary.PropositionalEquality as Eq
open Eq using (_≡_; refl; cong; sym)
open Eq.≡-Reasoning using (begin_; _≡⟨⟩_; step-≡; _∎)
open import Data.Nat using (ℕ; zero; suc; _+_; _*_; _∸_)

-- proof of assoc

+-assoc : ∀ (m n p : ℕ) → (m + n) + p ≡ m + (n + p)
+-assoc zero n p =
  begin
    (zero + n) + p
  ≡⟨⟩
    n + p
  ≡⟨⟩
    zero + (n + p)
  ∎

+-assoc (suc m) n p =
  begin
    (suc m + n) + p
  ≡⟨⟩
    suc (m + n) + p
  ≡⟨⟩
    suc ((m + n) + p)
  ≡⟨ cong suc (+-assoc m n p) ⟩
    suc (m + (n + p))
  ≡⟨⟩
    suc m + (n + p)
  ∎

-- proof of comm

+-identityʳ : ∀ (m : ℕ) → m + zero ≡ m
+-identityʳ zero =
  begin
    zero + zero
  ≡⟨⟩
    zero
  ∎

+-identityʳ (suc m) =
  begin
    (suc m) + zero
  ≡⟨⟩
    suc (m + zero)
  ≡⟨ cong suc (+-identityʳ m) ⟩
    suc m
  ∎

+-suc : ∀ (m n : ℕ) → m + suc n ≡ suc (m + n)
+-suc zero n =
  begin
    zero + suc n
  ≡⟨⟩
    suc n
  ≡⟨⟩
    suc (zero + n)
  ∎
+-suc (suc m) n =
  begin
    suc m + suc n
  ≡⟨⟩
    suc (m + suc n)
  ≡⟨ cong suc (+-suc m n) ⟩
    suc (suc (m + n))
  ≡⟨⟩
    suc (suc m + n)
  ∎

+-comm : ∀ (m n : ℕ) → m + n ≡ n + m
+-comm m zero =
  begin
    m + zero
  ≡⟨ +-identityʳ m ⟩
    m
  ≡⟨⟩
    zero + m
  ∎
+-comm m (suc n) =
  begin
    m + (suc n)
  ≡⟨ +-suc m n ⟩
    suc (m + n)
  ≡⟨ cong suc (+-comm m n) ⟩
    suc (n + m)
  ≡⟨⟩
    suc n + m
  ∎

-- coro

+-rearrange : ∀ (m n p q : ℕ) → (m + n) + (p + q) ≡ m + (n + p) + q
+-rearrange m n p q =
  begin
    (m + n) + (p + q)
  ≡⟨ +-assoc m n (p + q) ⟩
    m + (n + (p + q))
  ≡⟨ cong (m +_) (sym (+-assoc n p q)) ⟩
    m + ((n + p) + q)
  ≡⟨ sym (+-assoc m (n + p) q) ⟩
    (m + (n + p)) + q
  ∎

-- second proof of assoc with rewrite and refl

+-assoc′ : ∀ (m n p : ℕ) → (m + n) + p ≡ m + (n + p)
+-assoc′ zero n p = refl
+-assoc′ (suc m) n p rewrite +-assoc′ m n p = refl

-- second proof of comm with rewrite and refl

+-identity′ : ∀ (n : ℕ) → n + zero ≡ n
+-identity′ zero = refl
+-identity′ (suc n) rewrite +-identity′ n = refl

+-suc′ : ∀ (m n : ℕ) → m + suc n ≡ suc (m + n)
+-suc′ zero n = refl
+-suc′ (suc m) n rewrite +-suc′ m n = refl

+-comm′ : ∀ (m n : ℕ) → m + n ≡ n + m
+-comm′ m zero rewrite +-identity′ m = refl
+-comm′ m (suc n) rewrite +-suc′ m n
                        | +-comm′ m n
                        = refl

-- problems

+-swap : ∀ (m n p : ℕ) → m + (n + p) ≡ n + (m + p)
+-swap zero n p = refl
+-swap (suc m) n p rewrite +-assoc m n p
                         | +-comm m n
                         | +-swap m n p
                         | +-suc n (m + p)
                         = refl

*-distrib-+ : ∀ (m n p : ℕ) → (m + n) * p ≡ m * p + n * p
*-distrib-+ zero n p = refl
*-distrib-+ (suc m) n p rewrite *-distrib-+ m n p
                              | +-assoc p (m * p) (n * p)
                              = refl

*-assoc : ∀ (m n p : ℕ) → (m * n) * p ≡ m * (n * p)
*-assoc zero n p = refl
*-assoc (suc m) n p =
  begin
    ((suc m) * n) * p
  ≡⟨⟩
    (n + m * n) * p
  ≡⟨ *-distrib-+ n (m * n) p ⟩
    (n * p) + m * n * p
  ≡⟨ cong ((n * p) +_) (*-assoc m n p) ⟩
    (n * p) + m * (n * p)
  ≡⟨⟩
    (suc m) * (n * p)
  ∎
